end of day 11/07/19

inference-tool/src/main/scala/inference/Config.scala
@@ -1,0 +1,140 @@
+import scopt.OParser
+import java.io._
+import scala.io.Source
+import net.liftweb.json._
+import ch.qos.logback.classic.Level
+
+object Heuristics extends Enumeration {
+  type Heuristic = Value
+  val store, inc, same, ignore, ignoret, ignores = Value
+}
+
+object Nondeterminisms extends Enumeration {
+  type Nondeterminism = Value
+  val basic, labar = Value
+}
+
+object Strategies extends Enumeration {
+  type Strategy = Value
+  val naive, rank, comprehensive, comprehensiveEQ = Value
+}
+
+case class Config(
+  heuristics: Seq[Heuristics.Heuristic] = Seq(),
+  file: File = null,
+  outputname: String = null,
+  dotfiles: String = "dotfiles",
+  nondeterminism: Nondeterminisms.Nondeterminism = Nondeterminisms.basic,
+  strategy: Strategies.Strategy = Strategies.naive,
+  oneFinal: Boolean = false,
+  logLevel: Level = Level.DEBUG,
+  k: Int = 0
+)
+
+object Config {
+  val builder = OParser.builder[Config]
+
+  implicit val heuristicsRead: scopt.Read[Heuristics.Value] =
+    scopt.Read.reads(Heuristics withName _)
+  implicit val nondeterminismsRead: scopt.Read[Nondeterminisms.Value] =
+    scopt.Read.reads(Nondeterminisms withName _)
+  implicit val strategiesRead: scopt.Read[Strategies.Value] =
+    scopt.Read.reads(Strategies withName _)
+  implicit val booleanRead: scopt.Read[Level]     =
+  scopt.Read.reads { _.toLowerCase match {
+    case "debug"  => Level.DEBUG
+    case "warn"  => Level.WARN
+    case "info"  => Level.INFO
+    case "error"  => Level.ERROR
+    case s       =>
+      throw new IllegalArgumentException("'" + s + "' is not a boolean.")
+  }}
+
+  var config: Config = null
+  var log: List[List[TypeConversion.Event]] = List()
+  var strategy = (SelectionStrategies.naive_score _).curried
+  var heuristics = Inference.try_heuristics(List(), (Inference.nondeterministic_pairs _))
+  var nondeterminismMetric = (Inference.nondeterministic_pairs _)
+
+  val parser1 = {
+    import builder._
+    OParser.sequence(
+      programName("inference-tool"),
+      head("inference-tool", "0.x"),
+      help("help").text("prints this usage text"),
+      opt[Seq[Heuristics.Heuristic]]('h', "heuristics")
+        .valueName("<heuristic1>,<heuristic2>...")
+        .action((x, c) => c.copy(heuristics = x))
+        .text(s"heuristics to give the inference process ${Heuristics.values}"),
+      opt[String]('o', "output")
+        .valueName("filename")
+        .action((x, c) => c.copy(outputname = x))
+        .text("The preferred name of the file to output the SAL and DOT representations of the inferred model to - defaults to the input file name"),
+      opt[Int]('k', "k")
+        .valueName("k")
+        .action((x, c) => c.copy(k = x))
+        .text("The depth of the k-tails (defaults to zero)"),
+      opt[Strategies.Strategy]('s', "strategy")
+        .valueName("strategy")
+        .action((x, c) => c.copy(strategy = x))
+        .text(s"The preferred strategy to rank state merges ${Nondeterminisms.values}"),
+      opt[Nondeterminisms.Nondeterminism]('n', "nondeterminism")
+        .valueName("nondeterminism checker")
+        .action((x, c) => c.copy(nondeterminism = x))
+        .text(s"The preferred definition of nondeterminism - defaults to label, arity, and guard check ${Nondeterminisms.values}"),
+      opt[String]('d', "dotfiles")
+        .valueName("dir")
+        .action((x, c) => c.copy(dotfiles = x))
+        .text("The directory in which to save dotfiles produced during the inference process - defaults to 'dotfiles'"),
+      opt[Unit]("f1")
+        .action((_, c) => c.copy(oneFinal = true))
+        .text("Set this flag to merge states with no outgoing transitions"),
+      opt[Level]('l', "level")
+        .valueName("level")
+        .action((x, c) => c.copy(logLevel = x))
+        .text(s"The log level {info, debug, warn, error}"),
+      arg[File]("filename")
+        .required()
+        .action((x, c) => c.copy(file = x))
+        .text("The json file listing the traces"))
+  }
+
+  def parseArgs(args: Array[String]) = {
+    OParser.parse(parser1, args, Config()) match {
+      case Some(config) => {
+        this.config = config
+        val rawJson = Source.fromFile(config.file).getLines.mkString
+        val parsed = (parse(rawJson))
+        val list = parsed.values.asInstanceOf[List[List[Map[String, Any]]]]
+        this.log = list.map(run => run.map(x => TypeConversion.toEventTuple(x)))
+        val heuristics = scala.collection.immutable.Map(
+          Heuristics.store -> Store_Reuse.heuristic_1(log),
+          Heuristics.inc -> (Increment_Reset.insert_increment_2 _).curried,
+          Heuristics.same -> (Same_Register.same_register _).curried,
+          Heuristics.ignore -> (Ignore_Inputs.drop_inputs _).curried,
+          Heuristics.ignoret -> (Ignore_Inputs.transitionwise_drop_inputs _).curried,
+          Heuristics.ignores -> (Ignore_Inputs.statewise_drop_inputs _).curried)
+
+        val nondeterminisms = scala.collection.immutable.Map(
+          Nondeterminisms.basic -> (Inference.nondeterministic_pairs _),
+          Nondeterminisms.labar -> (Inference.nondeterministic_pairs_labar _))
+
+        val strategies = scala.collection.immutable.Map(
+          Strategies.naive -> (SelectionStrategies.naive_score _).curried,
+          Strategies.rank -> (SelectionStrategies.naive_score_outputs _).curried,
+          Strategies.comprehensive -> (SelectionStrategies.naive_score_comprehensive _).curried,
+          Strategies.comprehensiveEQ -> (SelectionStrategies.naive_score_comprehensive_eq_high _).curried)
+
+          this.strategy = strategies(config.strategy)
+        // this.strategy = if (Config.config.oneFinal)
+        //     (SelectionStrategies.score_one_final_state _).curried(strategies(config.strategy))
+        //   else (strategies(config.strategy))
+        this.heuristics = Inference.try_heuristics(config.heuristics.map(x => heuristics(x)).toList, nondeterminisms(config.nondeterminism))
+        this.nondeterminismMetric = nondeterminisms(config.nondeterminism)
+        }
+      case _ =>
+        System.exit(1)
+      }
+  }
+
+}
