inference-tool/src/main/scala/inference/FrontEnd.scala
@@ -1,142 +1,40 @@
-import net.liftweb.json._
 import scala.io.Source
 import com.microsoft.z3
 // PrintWriter
 import java.io._
 import org.apache.commons.io.FilenameUtils;
 import scala.collection.mutable.ListBuffer
-import scopt.OParser
-
-object Heuristics extends Enumeration {
-  type Heuristic = Value
-  val store, inc, same, ignore, ignoret, ignores = Value
-}
-
-object Nondeterminisms extends Enumeration {
-  type Nondeterminism = Value
-  val basic, labar = Value
-}
-
-object Strategies extends Enumeration {
-  type Strategy = Value
-  val naive, rank, comprehensive, comprehensiveEQ = Value
-}
 
 object FrontEnd {
-  case class Config(
-    heuristics: Seq[Heuristics.Heuristic] = Seq(),
-    file: File = null,
-    outputname: String = null,
-    dotfiles: String = "dotfiles",
-    nondeterminism: Nondeterminisms.Nondeterminism = Nondeterminisms.basic,
-    strategy: Strategies.Strategy = Strategies.naive,
-    oneFinal: Boolean = false
-  )
-
-  var config:Config = null
-
-  implicit val heuristicsRead: scopt.Read[Heuristics.Value] =
-    scopt.Read.reads(Heuristics withName _)
-  implicit val nondeterminismsRead: scopt.Read[Nondeterminisms.Value] =
-    scopt.Read.reads(Nondeterminisms withName _)
-  implicit val strategiesRead: scopt.Read[Strategies.Value] =
-    scopt.Read.reads(Strategies withName _)
-
   def main(args: Array[String]): Unit = {
-    val builder = OParser.builder[Config]
-    val parser1 = {
-      import builder._
-      OParser.sequence(
-        programName("inference-tool"),
-        head("inference-tool", "0.x"),
-        help("help").text("prints this usage text"),
-        opt[Seq[Heuristics.Heuristic]]('h', "heuristics")
-          .valueName("<heuristic1>,<heuristic2>...")
-          .action((x, c) => c.copy(heuristics = x))
-          .text(s"heuristics to give the inference process ${Heuristics.values}"),
-        opt[String]('o', "output")
-          .valueName("filename")
-          .action((x, c) => c.copy(outputname = x))
-          .text("The preferred name of the file to output the SAL and DOT representations of the inferred model to - defaults to the input file name"),
-        opt[Strategies.Strategy]('s', "strategy")
-            .valueName("strategy")
-            .action((x, c) => c.copy(strategy = x))
-            .text(s"The preferred strategy to rank state merges ${Nondeterminisms.values}"),
-        opt[Nondeterminisms.Nondeterminism]('n', "nondeterminism")
-          .valueName("nondeterminism checker")
-          .action((x, c) => c.copy(nondeterminism = x))
-          .text(s"The preferred definition of nondeterminism - defaults to label, arity, and guard check ${Nondeterminisms.values}"),
-        opt[String]('d', "dotfiles")
-            .valueName("dir")
-            .action((x, c) => c.copy(dotfiles = x))
-            .text("The directory in which to save dotfiles produced during the inference process - defaults to 'dotfiles'"),
-        opt[Unit]("f1")
-            .action((_, c) => c.copy(oneFinal = true))
-            .text("Set this flag to merge states with no outgoing transitions"),
-        arg[File]("filename")
-          .required()
-          .action((x, c) => c.copy(file = x))
-          .text("The json file listing the traces"))
-    }
 
-    println("=================================================================")
     val t1 = System.nanoTime
-    OParser.parse(parser1, args, Config()) match {
-      case Some(config) =>
-        this.config = config
-        val rawJson = Source.fromFile(config.file).getLines.mkString
-        val parsed = (parse(rawJson))
-        val list = parsed.values.asInstanceOf[List[List[Map[String, Any]]]]
-        val log = list.map(run => run.map(x => TypeConversion.toEventTuple(x)))
+    Config.parseArgs(args)
 
-        val heuristics = scala.collection.immutable.Map(
-          Heuristics.store -> Store_Reuse.heuristic_1(log),
-          Heuristics.inc -> (Increment_Reset.insert_increment_2 _).curried,
-          Heuristics.same -> (Same_Register.same_register _).curried,
-          Heuristics.ignore -> (Ignore_Inputs.drop_inputs _).curried,
-          Heuristics.ignoret -> (Ignore_Inputs.transitionwise_drop_inputs _).curried,
-          Heuristics.ignores -> (Ignore_Inputs.statewise_drop_inputs _).curried
-        )
+    Log.root.info("Building PTA")
+    val pta = Inference.make_pta(Config.log, FSet.bot_fset)
+    TypeConversion.efsmToSALTranslator(pta, "pta")
+    PrettyPrinter.EFSM2dot(pta, s"pta_gen")
 
-        val nondeterminisms = scala.collection.immutable.Map(
-          Nondeterminisms.basic -> (Inference.nondeterministic_pairs _),
-          Nondeterminisms.labar -> (Inference.nondeterministic_pairs_labar _)
-        )
+    val np_labar = Inference.nondeterministic_pairs_labar(Inference.toiEFSM(pta))
 
-        val strategies = scala.collection.immutable.Map(
-          Strategies.naive -> (SelectionStrategies.naive_score _).curried,
-          Strategies.rank -> (SelectionStrategies.naive_score_rank _).curried,
-          Strategies.comprehensive -> (SelectionStrategies.naive_score_comprehensive _).curried,
-          Strategies.comprehensiveEQ -> (SelectionStrategies.naive_score_comprehensive_eq_high _).curried
-        )
+    val inferred = Inference.learn(
+      Nat.Nata(Config.config.k),
+      Config.log,
+      Config.strategy,
+      Config.heuristics,
+      Config.nondeterminismMetric)
 
-        println("Building PTA")
-        val pta = Inference.make_pta(log, FSet.bot_fset)
-        // TypeConversion.efsmToSALTranslator(pta, "pta")
-        val np_labar = Inference.nondeterministic_pairs_labar(Inference.toiEFSM(pta))
+    Log.root.info("The inferred machine is " +
+      (if (Inference.nondeterministic(Inference.toiEFSM(inferred), Inference.nondeterministic_pairs)) "non" else "") + "deterministic")
 
-        val inferred = Inference.learn(
-          log,
-          if (config.oneFinal)
-            (SelectionStrategies.score_one_final_state _).curried(strategies(config.strategy))
-          else (strategies(config.strategy)),
-          Inference.try_heuristics(config.heuristics.map(x => heuristics(x)).toList, nondeterminisms(config.nondeterminism)),
-          nondeterminisms(config.nondeterminism))
+    val basename = (if (Config.config.outputname == null) (FilenameUtils.getBaseName(Config.config.file.getName()).replace("-", "_")) else Config.config.outputname.replace("-", "_"))
+    TypeConversion.efsmToSALTranslator(inferred, basename)
 
-            println("The inferred machine is " +
-              (if (Inference.nondeterministic(Inference.toiEFSM(inferred), Inference.nondeterministic_pairs)) "non" else "") + "deterministic")
-            println(Inference.nondeterministic_pairs(Inference.toiEFSM(inferred)))
-
-            val basename = (if (config.outputname == null) (FilenameUtils.getBaseName(config.file.getName()).replace("-", "_")) else config.outputname.replace("-", "_"))
-
-            TypeConversion.efsmToSALTranslator(inferred, basename)
-      case _ =>
-        System.exit(1)
-    }
+    PrettyPrinter.EFSM2dot(inferred, s"${basename}_gen")
     val seconds = (System.nanoTime - t1) / 1e9d
-    val minutes = (seconds/60)%60
-    val hours = seconds/3600
-    println(s"Completed in ${if (hours > 0) s"${hours.toInt}h " else ""}${if (minutes > 0) s"${minutes.toInt}m " else ""}${seconds%60}s")
-    println("=================================================================")
+    val minutes = (seconds / 60) % 60
+    val hours = seconds / 3600
+    Log.root.info(s"Completed in ${if (hours > 0) s"${hours.toInt}h " else ""}${if (minutes > 0) s"${minutes.toInt}m " else ""}${seconds % 60}s")
   }
 }
