inference-tool/src/main/scala/inference/Log.scala
@@ -1,0 +1,13 @@
+import org.slf4j.LoggerFactory
+import ch.qos.logback.classic.Level
+import ch.qos.logback.classic.Logger
+
+object Log {
+  val root =  LoggerFactory.getLogger("root").asInstanceOf[Logger]
+  root.setLevel(Config.config.logLevel)
+
+  def logStates(s_1: Nat.nat, s_2: Nat.nat) = {
+    root.debug(s"${Code_Numeral.integer_of_nat(s_2)} -> ${Code_Numeral.integer_of_nat(s_1)}")
+  }
+
+}
