formal/inference/SelectionStrategies.thy
@@ -6,56 +6,41 @@ theory SelectionStrategies
 imports Inference
 begin
 
-subsection\<open>One of the simplest strategies is to look only at the labels and arities of outgoing
-transitions of each state. Pairs of states are ranked by how many transitions with the same label
-and arity they have in common.\<close>
-definition naive_score :: strategy where
-  "naive_score t1 t2 = size (ffilter (\<lambda>(x, y). Label x = Label y \<and> Arity x = Arity y) (t1 |\<times>| t2))"
-
-lemma naive_score_empty: "\<forall>a. naive_score a {||} = 0"
-  by (simp add: naive_score_def)
-
-lemma naive_score_empty_2: "\<forall>a. naive_score {||} a = 0"
-  by (simp add: naive_score_def)
-
-definition score_one_final_state :: "strategy \<Rightarrow> strategy" where
-  "score_one_final_state s t1 t2 = (if t1 = {||} \<and> t2 = {||} then 1 else s t1 t2)"
-
-definition naive_score_one_final_state :: strategy where
-  "naive_score_one_final_state = score_one_final_state naive_score"
-
 fun bool2nat :: "bool \<Rightarrow> nat" where
   "bool2nat True = 1" |
   "bool2nat False = 0"
 
-(* One point each for equal label, arity, and outputs *)
-definition naive_score_rank :: strategy where
-  "naive_score_rank t1 t2 = Sum (fset (fimage (\<lambda>(x, y). bool2nat (Label x = Label y) + bool2nat (Arity x = Arity y) + bool2nat (Outputs x = Outputs y)) (t1 |\<times>| t2)))"
+subsection\<open>One of the simplest strategies is to look only at the labels and arities of outgoing
+transitions of each state. Pairs of states are ranked by how many transitions with the same label
+and arity they have in common.\<close>
+definition naive_score :: strategy where
+  "naive_score t1 t2 = bool2nat (Label t1 = Label t2 \<and> Arity t1 = Arity t2)"
 
-definition naive_score_rank_one_final_state :: strategy where
-  "naive_score_rank_one_final_state = score_one_final_state naive_score_rank"
+(* One point if they're equal *)
+definition naive_score_eq :: strategy where
+  "naive_score_eq t1 t2 = bool2nat (t1 = t2)"
+
+(* One point each for equal label, arity, and outputs *)
+definition naive_score_outputs :: strategy where
+  "naive_score_outputs x y = bool2nat (Label x = Label y) + bool2nat (Arity x = Arity y) + bool2nat (Outputs x = Outputs y)"
 
 (* Functions with same label, and input and output arities contribute one point for each guard    *)
 (* and output they share. *)
 definition naive_score_comprehensive :: strategy where
-  "naive_score_comprehensive t1 t2 = Sum (fset (fimage (\<lambda>(x, y). if Label x = Label y \<and> Arity x = Arity y then
-                                                                   if length (Outputs x) = length (Outputs y) then
-                                                                     card (set (Guard x) \<inter> set (Guard y)) + length (filter (\<lambda>(p1, p2). p1 = p2) (zip (Outputs x) (Outputs y)))
-                                                                   else 0
-                                                                 else 0)
-                                               (t1 |\<times>| t2)))"
+  "naive_score_comprehensive x y = (if Label x = Label y \<and> Arity x = Arity y then
+                                      if length (Outputs x) = length (Outputs y) then
+                                       card (set (Guard x) \<inter> set (Guard y)) + length (filter (\<lambda>(p1, p2). p1 = p2) (zip (Outputs x) (Outputs y)))
+                                     else 0
+                                   else 0)"
 
 (* Functions with same label, and input and output arities contribute one point for each guard    *)
 (* and output they share. Transitions which are exactly equal get a very high score. *)
 definition naive_score_comprehensive_eq_high :: strategy where
-  "naive_score_comprehensive_eq_high t1 t2 = Sum (fset (fimage (\<lambda>(x, y). 
-                                                               if x = y then 100 else
-                                                                 if Label x = Label y \<and> Arity x = Arity y then
-                                                                   if length (Outputs x) = length (Outputs y) then
-                                                                     card (set (Guard x) \<inter> set (Guard y)) + length (filter (\<lambda>(p1, p2). p1 = p2) (zip (Outputs x) (Outputs y)))
-                                                                   else 0
-                                                                 else 0)
-                                               (t1 |\<times>| t2)))"
-
+  "naive_score_comprehensive_eq_high x y = (if x = y then 100 else
+                                             if Label x = Label y \<and> Arity x = Arity y then
+                                               if length (Outputs x) = length (Outputs y) then
+                                                 card (set (Guard x) \<inter> set (Guard y)) + length (filter (\<lambda>(p1, p2). p1 = p2) (zip (Outputs x) (Outputs y)))
+                                               else 0
+                                             else 0)"
 
 end
